---
title: "Deriving the Ridge Solution"
author: "Dr. D'Agostino McGowan"
output:
  xaringan::moon_reader:
    css: "slides.css"
    logo: img/icon.png
    lib_dir: libs
    nature:
      highlightStyle: github
      highlightLines: true
      countIncrementalSlides: false
---



```{r child = "setup.Rmd"}
```

layout: true

<div class="my-footer">
  <span>
  Dr. Lucy D'Agostino McGowan
</span>
</div> 

---

## Ridge Regression

* Foil!

$$\begin{align}
&RSS + \lambda\beta^T\beta\\
\end{align}$$

---

## Ridge Regression

* Foil!

$$\begin{align}
&RSS + \lambda\beta^T\beta\\
&(\mathbf{y}-\mathbf{X}\beta)^T(\mathbf{y}-\mathbf{X}\beta)+\lambda\beta^T\beta\\
\end{align}$$

---
## Ridge Regression

* Foil!

$$\begin{align}
&RSS + \lambda\beta^T\beta\\
&(\mathbf{y}-\mathbf{X}\beta)^T(\mathbf{y}-\mathbf{X}\beta)+\lambda\beta^T\beta\\
&\mathbf{y}^T\mathbf{y}-2\beta^T\mathbf{X}^T\mathbf{y}+\beta^T\mathbf{X}^T\mathbf{X}\beta+\lambda\beta^T\beta\\
\end{align}$$

---

## Ridge Regression

* Take the derivative

$$\frac{\partial \mathbf{y}^T\mathbf{y}-2\beta^T\mathbf{X}^T\mathbf{y}+\beta^T\mathbf{X}^T\mathbf{X}\beta+\lambda\beta^T\beta}{\partial\beta}$$
--

$$-2\mathbf{X}^T\mathbf{y}+2\mathbf{X}^T\mathbf{X}\beta+2\lambda\beta$$

---

## Ridge Regression 

* Set it equal to 0, solve for $\beta$

$$\begin{align}0 &= -2\mathbf{X}^T\mathbf{y}+2\mathbf{X}^T\mathbf{X}\beta+2\lambda\beta\\
\end{align}$$
---

## Ridge Regression 

* Set it equal to 0, solve for $\beta$

$$\begin{align}0 &= -2\mathbf{X}^T\mathbf{y}+2\mathbf{X}^T\mathbf{X}\beta+2\lambda\beta\\
0&=-\mathbf{X}^T\mathbf{y}+\mathbf{X}^T\mathbf{X}\beta+\lambda\beta\\
\end{align}$$
---

## Ridge Regression 

* Set it equal to 0, solve for $\beta$

$$\begin{align}0 &= -2\mathbf{X}^T\mathbf{y}+2\mathbf{X}^T\mathbf{X}\beta+2\lambda\beta\\
0&=-\mathbf{X}^T\mathbf{y}+\mathbf{X}^T\mathbf{X}\beta+\lambda\beta\\
\mathbf{X}^T\mathbf{y}&=\mathbf{X}^T\mathbf{X}\beta+\lambda\beta\\
\end{align}$$
---

## Ridge Regression 

* Set it equal to 0, solve for $\beta$

$$\begin{align}0 &= -2\mathbf{X}^T\mathbf{y}+2\mathbf{X}^T\mathbf{X}\beta+2\lambda\beta\\
0&=-\mathbf{X}^T\mathbf{y}+\mathbf{X}^T\mathbf{X}\beta+\lambda\beta\\
\mathbf{X}^T\mathbf{y}&=\mathbf{X}^T\mathbf{X}\beta+\lambda\beta\\
\mathbf{X}^T\mathbf{y}&=(\mathbf{X}^T\mathbf{X}+\lambda\mathbf{I})\beta
\end{align}$$

---

## Ridge Regression 

* Set it equal to 0, solve for $\beta$

$$\begin{align}0 &= -2\mathbf{X}^T\mathbf{y}+2\mathbf{X}^T\mathbf{X}\beta+2\lambda\beta\\
0&=-\mathbf{X}^T\mathbf{y}+\mathbf{X}^T\mathbf{X}\beta+\lambda\beta\\
\mathbf{X}^T\mathbf{y}&=\mathbf{X}^T\mathbf{X}\beta+\lambda\beta\\
\mathbf{X}^T\mathbf{y}&=(\mathbf{X}^T\mathbf{X}+\lambda\mathbf{I})\beta\\
(\mathbf{X}^T\mathbf{X}+\lambda\mathbf{I})^{-1}\mathbf{X}^T\mathbf{y}&=\beta
\end{align}$$
